src/Pipit.Exp.Bigstep.fst
@@ -284,3 +284,19 @@ let bigstep_deterministic
     Lemma (ensures (v1 == v2)) (decreases hBS1) =
   bigstep_proof_equivalence hBS1 hBS2
 
+
+let bigstep_deterministic_squash
+  (#t: table)
+  (#c: context t)
+  (streams: list (row c))
+  (#a: t.ty)
+  (e: exp t c a)
+  (v1 v2: t.ty_sem a):
+    Lemma
+      (requires (bigstep streams e v1 /\ bigstep streams e v2))
+      (ensures (v1 == v2)) =
+  FStar.Squash.bind_squash #(bigstep streams e v1) ()
+    (fun (a: bigstep streams e v1) ->
+  FStar.Squash.bind_squash #(bigstep streams e v2) #(v1 == v2) ()
+    (fun (b: bigstep streams e v2) ->
+      bigstep_deterministic a b))
